\documentclass{article}
\usepackage[utf8]{vietnam}
\usepackage{amsmath,amssymb}
 

\begin{document}
\noindent
\textbf{\textsl{3.1-1}}
Let $f(n)$ and $g(n)$ be asymptotically nonnegative functions. Using the basic definition of $\Theta$-notation,
prove that $\max\left(f(n), g(n)\right) = \Theta(f(n) + g(n))$.
\newline
\newline
%\hline

If we allow us to reframe the question. Define
\begin{align*}
	h \!:\quad n \;&\mapsto\quad \max(f(n), g(n)) \\
	l \!:\quad n \;&\mapsto\quad f(n) + g(n)
\end{align*}
Then we are supposed to show that $h(n) = \Theta(l(n))$.

\noindent
Since $f$ and $g$ are asymtotically nonnegative, we have
\begin{align*}
	& \exists\; n_1 \quad\textrm{s.t.}\quad f(n) \ge 0 \quad\forall\; n \ge n_1 \\
	& \exists\; n_2 \quad\textrm{s.t.}\quad g(n) \ge 0 \quad\forall\; n \ge n_2
\end{align*}
Let $n_3 = \max(n_1, n_2)$. Then for the constants $c_1=\frac{1}{2}, c_2=1, n_3$, we see that
\begin{align*}
	c_1 l(n) &\le h(n) \le c_2 l(n) \quad\forall\; n \ge n_3\,, \quad \textrm{i.e.}\\
	\frac{1}{2}(f(n) + g(n)) &\le \max\left(f(n), g(n)\right) \le f(n) + g(n) \quad\forall\; n \ge n_3\,.
\end{align*}
\hfill$\blacksquare$

\end{document}
